Add tests for reference equality, which previously didn't pass but now do

Test/traits/TraitCompile.dfy
@@ -92,6 +92,8 @@ method Main()
 
   NonCapturingFunctionCoercions.Test();
   TailRecursion.Test();
+
+  ObjectEquality.Test();
 }
 
 module OtherModule {
@@ -738,5 +740,61 @@ module TailRecursion {
     var y := c.Compute(15, 1_000_000);
     var z := c.Compute(15, 999_999);
     print x, " ", y, " ", z, "\n";  // 41 15 26
+  }
+}
+
+module ObjectEquality {
+  method Test() {
+    TestReferenceEquality();
+    NotTheSame();
+    TestSequences();
+  }
+
+  trait A { }
+
+  trait B extends A { }
+
+  class C extends B { }
+  class D extends B { }
+
+  method TestReferenceEquality() {
+    var c: C := new C;
+    var b: B := c;
+    var a0: A := c;
+    var a1: A := c;
+
+    print a0 == a1, " ", Eq(a0, a1), "\n";
+    print a0 == c, " ", Eq(a0, c), "\n";
+    print b == c, " ", Eq(b, c), "\n";
+    print b == a0, " ", Eq(b, a0), "\n";
+  }
+
+  predicate method Eq<U(==)>(u: U, v: U) {
+    u == v
+  }
+
+  method NotTheSame() {
+    var c: C, d: D := new C, new D;
+    var oc: object, od: object := c, d;
+
+    print oc != od, " ", !Eq(oc, od), " ", !Eq(c, d), "\n";
+
+    var ac: A, ad: A := c, d;
+    print ac != ad, " ", !Eq(ac, ad), " ", !Eq(ac, ad), "\n";
+  }
+
+  method TestSequences() {
+    /** TODO: Include this when all compilers support seq<TRAIT>
+    var c: C := new C;
+    var b: B := c;
+    var a: A := c;
+
+    var s: seq<A> := [a];
+    var t: seq<B> := [b];
+    var u: seq<C> := [c];
+
+    print s == t, " ", t == u, " ", u == s, "\n";
+    print s[0] == t[0], " ", t[0] == u[0], " ", u[0] == s[0], "\n";
+    **/
   }
 }
